src/example/treiber/Code.v
@@ -10,16 +10,12 @@ Module TreiberStack.
     Context {ident : ID}.
 
     Definition push_loop :
-      (* ktree (threadE void unit) (SCMem.val * SCMem.val) unit *)
-      ktree (threadE ident state) (SCMem.val * SCMem.val) unit
-      :=
-      fun '(s, node) =>
-        ITree.iter
-          (fun (_ : unit) =>
-             head <- (OMod.call (R:=SCMem.val) "load" s);;
-             _ <- (OMod.call (R:=unit) "store" (node,head));;
-             b <- (OMod.call (R:=bool) "cas" (s, head, node));;
-             if b then Ret (inr tt) else Ret (inl tt)) tt.
+      ktree (threadE ident state) (SCMem.val * SCMem.val) (unit + unit)
+      := fun '(s, node) =>
+        head <- (OMod.call (R:=SCMem.val) "load" s);;
+        _ <- (OMod.call (R:=unit) "store" (node,head));;
+        b <- (OMod.call (R:=bool) "cas" (s, head, node));;
+        if b then Ret (inr tt) else Ret (inl tt).
 
     Definition push :
       (* ktree (threadE void unit) (SCMem.val * SCMem.val) unit *)
@@ -28,8 +24,24 @@ Module TreiberStack.
       fun '(s,val) =>
         node <- (OMod.call (R:=SCMem.val) "alloc" 2);;
         _ <- (OMod.call (R:=unit) "store" (SCMem.val_add node 1, val));;
-        _ <- push_loop (s, node);;
+        _ <- ITree.iter (fun (_ : unit) => push_loop (s, node)) tt;;
         trigger Yield.
+
+    Definition pop_loop :
+      ktree (threadE ident state) SCMem.val (unit + option (SCMem.val))
+      :=
+      fun s =>
+        head <- (OMod.call (R:=SCMem.val) "load" s);;
+        is_null <- (OMod.call (R:=bool) "compare" (head, SCMem.val_null));;
+        if is_null then Ret (inr None) else
+        next <- (OMod.call (R:=SCMem.val) "load" head);;
+        b <- (OMod.call (R:=bool) "cas" (s, head, next));;
+        if b then
+          data <- (OMod.call (R:=SCMem.val) "load" (SCMem.val_add head 1));;
+          Ret (inr (Some data))
+        else
+          Ret (inl tt)
+        .
 
     Definition pop :
       (* ktree (threadE void unit) SCMem.val (option (SCMem.val) *)
@@ -37,20 +49,7 @@ Module TreiberStack.
       :=
       fun s =>
         _ <- trigger Yield;;
-        ITree.iter
-          (fun (_ : unit) =>
-            head <- (OMod.call (R:=SCMem.val) "load" s);;
-            is_null <- (OMod.call (R:=bool) "compare" (head, SCMem.val_null));;
-            if is_null then Ret (inr None) else (
-              next <- (OMod.call (R:=SCMem.val) "load" head);;
-              b <- (OMod.call (R:=bool) "cas" (s, head, next));;
-              if b then
-                data <- (OMod.call (R:=SCMem.val) "load" (SCMem.val_add head 1));;
-                Ret (inr (Some data))
-              else
-                Ret (inl tt)
-            )
-          ) tt.
+        ITree.iter (fun (_ : unit) => pop_loop s) tt.
 
     (** TODO : more rules for module composition. *)
     (* Definition omod : Mod.t := *)
