src/example/treiber/SpecHOCAP.v
@@ -2,30 +2,20 @@ From sflib Require Import sflib.
 From Paco Require Import paco.
 Require Import Coq.Classes.RelationClasses Lia Program.
 From iris Require Import bi.big_op.
-From Fairness Require Import pind Axioms ITreeLib Red TRed IRed2 WFLibLarge.
+From Fairness Require Import pind ITreeLib Red TRed IRed2 WFLibLarge.
 From Fairness Require Import FairBeh Mod Linking.
 From Fairness Require Import treiber.Code.
 From Fairness Require Import PCM IProp IPM IPropAux.
 From Fairness Require Import IndexedInvariants OpticsInterp SimWeakest.
 From Fairness Require Import TemporalLogic SCMemSpec ghost_var ghost_map.
 
-Record maybe_null_ptr := {
-  ptr :> SCMem.val;
-  ptr_mabye_null : ptr = SCMem.val_null \/ (∃ (p : SCMem.pointer), ptr = SCMem.val_ptr p);
-}.
+Inductive maybe_null_ptr :=
+| Null
+| Ptr (p : SCMem.pointer)
+.
+
 Global Instance maybe_null_ptr_eq_dec : EqDecision maybe_null_ptr.
-Proof.
-  intros [p1 Pp1] [p2 Pp2].
-  unfold Decision. destruct (decide (p1 = p2)) as [->|NEQ].
-  - left. f_equal. apply proof_irrelevance.
-  - right. intros H. apply NEQ. injection H. done.
-Qed.
-
-Definition to_mnp_null : maybe_null_ptr := {| ptr := SCMem.val_null; ptr_mabye_null := or_introl eq_refl |}.
-
-Definition to_mnp_ptr ptr
-  (IsPtr : (∃ (p : SCMem.pointer), ptr = SCMem.val_ptr p)) :=
-  {| ptr := ptr; ptr_mabye_null := or_intror IsPtr |}.
+Proof. solve_decision. Qed.
 
 Section SPEC.
 
@@ -50,12 +40,17 @@ Section SPEC.
   Ltac red_tl_all := red_tl_every; red_tl_memra; red_tl_ghost_var_ura; red_tl_ghost_map_ura.
 
   Definition to_val (mnp : maybe_null_ptr) : SCMem.val :=
-    ptr mnp.
+    match mnp with
+    | Null => SCMem.val_null
+    | Ptr p => SCMem.val_ptr p
+    end
+    .
 
   Fixpoint phys_list n (l : maybe_null_ptr) (L : list SCMem.val) : sProp n := (
-    match L with
-    | [] => ⌜to_val l = SCMem.val_null⌝
-    | v::tL => ∃ (p : τ{SCMem.pointer}) (r : τ{maybe_null_ptr}), ⌜to_val l = SCMem.val_ptr p⌝ ∗ (l ↦∗□ [(to_val r); v]) ∗ (phys_list n r tL)
+    match L,l with
+    | [],Null => emp
+    | v::tL,Ptr p => ∃ (r : τ{maybe_null_ptr}), (p ↦∗□ [(to_val r); v]) ∗ (phys_list n r tL)
+    | _,_ => ⌜False⌝
     end
   )%S.
 
@@ -92,10 +87,10 @@ Section SPEC.
   Qed.
 
   Lemma Inv_unfold n s k γs γl :
-    (⟦ Inv n s k γs γl, n ⟧) -∗
-    (∃ (h : τ{maybe_null_ptr,n}) (L : τ{list SCMem.val,n}) (m : τ{gmap nat maybe_null_ptr,n}),
+    ⟦ Inv n s k γs γl, n ⟧ -∗
+    ∃ h L m,
       (s ↦ (to_val h)) ∗ ghost_var γs (1/2) L ∗
-      ⟦ (phys_list n h L), n⟧ ∗ ⟦ LInv n k γl h m, n⟧).
+      ⟦ phys_list n h L, n⟧ ∗ ⟦ LInv n k γl h m, n⟧.
   Proof.
     unfold Inv. iIntros "Inv".
     repeat (red_tl; iDestruct "Inv" as "[% Inv]").
@@ -104,8 +99,8 @@ Section SPEC.
 
   Lemma Inv_fold n s k γs γl h L m :
     (s ↦ (to_val h)) -∗ ghost_var γs (1/2) L -∗
-    ⟦ (phys_list n h L), n⟧ -∗ ⟦ LInv n k γl h m, n⟧
-    -∗ (⟦ Inv n s k γs γl, n ⟧).
+    ⟦ phys_list n h L, n⟧ -∗ ⟦ LInv n k γl h m, n⟧
+    -∗ ⟦ Inv n s k γs γl, n ⟧.
   Proof.
     unfold Inv. iIntros "? ? ? ?".
     repeat (red_tl; iExists _).
@@ -113,7 +108,7 @@ Section SPEC.
   Qed.
 
   Lemma LInv_unfold n k γs h m :
-    (⟦ LInv n k γs h m, n ⟧) -∗
+    ⟦ LInv n k γs h m, n ⟧ -∗
     ghost_map_auth γs 1 m ∗
     [∗ map] a ∈ m,
       if decide (h = a) then
@@ -136,7 +131,7 @@ Section SPEC.
         else
           ◇[k](0, 1)
         )
-    -∗ (⟦ LInv n k γl h m, n ⟧).
+    -∗ ⟦ LInv n k γl h m, n ⟧.
   Proof.
     unfold LInv. red_tl_all. iIntros "$ H".
     rewrite red_syn_big_sepM.
@@ -146,45 +141,44 @@ Section SPEC.
 
 
   Lemma phys_list_unfold n l L :
-    (⟦ phys_list n l L, n ⟧) -∗
-    match L with
-    | [] => ⌜to_val l = SCMem.val_null⌝
-    | v::tL => ∃ (p : τ{SCMem.pointer,n}) (r : τ{maybe_null_ptr,n}), ⌜to_val l = SCMem.val_ptr p⌝ ∗ (l ↦∗□ [(to_val r); v]) ∗ (⟦phys_list n r tL,n⟧)
+    ⟦ phys_list n l L, n ⟧ -∗
+    match L,l with
+    | [],Null => emp
+    | v::tL,Ptr p => ∃ r, (p ↦∗□ [(to_val r); v]) ∗ ⟦phys_list n r tL,n⟧
+    | _,_ => ⌜False⌝
     end.
   Proof.
-    iIntros "H". des_ifs. simpl.
-    red_tl_all; iDestruct "H" as "[%x H]".
-    red_tl_all; iDestruct "H" as "[%r H]".
-    red_tl_all; iDestruct "H" as "[%EQ [(l.n↦ & l.d↦ & _) Phys]]".
-    iExists _,_. iFrame. done.
+    iIntros "H". des_ifs. simpl. destruct p.
+    red_tl_all; iDestruct "H" as (r) "H".
+    red_tl_all; iDestruct "H" as "[(l.n↦ & l.d↦ & _) Phys]".
+    iExists _. iFrame.
   Qed.
 
   Lemma phys_list_fold n l L :
-    (match L with
-    | [] => ⌜to_val l = SCMem.val_null⌝
-    | v::tL => ∃ (p : τ{SCMem.pointer,n}) (r : τ{maybe_null_ptr,n}), ⌜to_val l = SCMem.val_ptr p⌝ ∗ (l ↦∗□ [(to_val r); v]) ∗ (⟦phys_list n r tL,n⟧)
-    end) -∗
+    match L,l with
+    | [],Null => emp
+    | v::tL,Ptr p => ∃ r, (p ↦∗□ [(to_val r); v]) ∗ ⟦phys_list n r tL,n⟧
+    | _,_ => ⌜False⌝
+    end -∗
     ⟦ phys_list n l L, n ⟧.
   Proof.
-    iIntros "H". des_ifs. simpl.
-    red_tl_all; iDestruct "H" as "[%x [%r [%EQ [(l.n↦ & l.d↦ & _) Phys]]]]".
-    red_tl_all. iExists x. red_tl_all. iExists r.
-    red_tl_all. iFrame. done.
+    iIntros "H". des_ifs. simpl. destruct p.
+    red_tl_all; iDestruct "H" as (r) "[(l.n↦ & l.d↦ & _) Phys]".
+    red_tl_all. iExists r.
+    red_tl_all. iFrame.
   Qed.
 
   Lemma phys_list_get_head n l L :
     ⟦ phys_list n l L, n ⟧ -∗
-    □ if (decide (to_val l = SCMem.val_null)) then
+    □ if decide (l = Null) then
         emp
-      else (∃ (r : τ{maybe_null_ptr,n}) (h : τ{SCMem.val,n}),
-                 (l ↦∗□ [(to_val r); h]))
+      else ∃ r h, (to_val l ↦∗□ [(to_val r); h])
     .
   Proof.
-    iIntros "H". iDestruct (phys_list_unfold with "H") as "H". destruct L; try done.
-    all: case_decide; try done.
-    - iDestruct "H" as %EQ. done.
-    - iDestruct "H" as (p r) "[%EQ [#H _]]".
-      red_tl_all. iExists r, v. iFrame "H".
+    iIntros "H". iDestruct (phys_list_unfold with "H") as "H".
+    des_ifs.
+    iDestruct "H" as (r) "[#H _]".
+    iExists r, v. iFrame "H".
   Qed.
 
   Lemma alloc_Treiber n s l a :
@@ -198,7 +192,7 @@ Section SPEC.
     iEval (rewrite ghost_var_split) in "V".
     iDestruct "V" as "[VI VS]".
     iMod (FUpd_alloc _ _ _ n (treiberN) (Inv n s k γs γl) with "[VI s↦ M]") as "#Inv"; [lia| |].
-    { iApply (Inv_fold _ _ _ _ _ to_mnp_null with "s↦ VI [] [M]").
+    { iApply (Inv_fold _ _ _ _ _ Null with "s↦ VI [] [M]").
       - iApply phys_list_fold. done.
       - iApply (LInv_fold with "M"). done.
     }
@@ -223,10 +217,12 @@ Section SPEC.
             Q ∗ (⤉ Duty(tid) ds)
             )%S, 1+n⟧⧽
   .
-  Proof.
+  Proof using DISJ.
+    Local Opaque TreiberStack.push_loop.
     ii. iStartTriple. red_tl_all.
     unfold IsT,TStack. rewrite red_syn_tgt_interp_as. rewrite red_syn_atomic_update. red_tl. simpl.
-    iIntros "(#Mem & IsT & Duty & AU & Ob_ks & PCS) Post".
+    iIntros "(#Mem & IsT & Duty & AU & Ob_ks & PCS)".
+    set POST := (POST in (POST -∗ _)%I). iIntros "Post".
     iDestruct "IsT" as (γl) "IsT".
     red_tl. rewrite red_syn_inv. iDestruct "IsT" as "#[Ob_kb IsT]".
 
@@ -263,8 +259,14 @@ Section SPEC.
         - iApply ("Ind" with "PCS").
     }
 
-    iModIntro. iExists 0. iIntros "IH !> Pcs %next n.n↦ Post Duty Ys AU n.d↦ Ob_ks".
-    iEval (rewrite unfold_iter_eq). rred2r.
+    iModIntro. iExists 0.
+    set IH := (IH in (IH ==∗ _)%I).
+    iIntros "IH !> Pcs %next n.n↦ Post Duty Ys AU n.d↦ Ob_ks".
+    iEval (rewrite unfold_iter_eq).
+    Local Transparent TreiberStack.push_loop.
+    rred2r.
+    fold (TreiberStack.push_loop (state := Mod.state Client) (ident := Mod.ident Client) (s,node)).
+    Local Opaque TreiberStack.push_loop.
     iMod (pcs_decr _ _ 97 1 with "Ys") as "[Ys Y]"; [lia|].
 
     iApply (wpsim_yieldR with "[$Y $Duty]"); [lia|].
@@ -333,10 +335,9 @@ Section SPEC.
       (* Update physical stack state. *)
       iMod (SCMem.points_to_persist with "n.n↦") as "#n.n↦".
       iMod (SCMem.points_to_persist with "n.d↦") as "#n.d↦".
-      iAssert (⌜∃ p : τ{SCMem.pointer,n}, node = SCMem.val_ptr p⌝)%I as %IsPtr.
-      { destruct node; try done. iPureIntro. eauto. }
-      iAssert (⟦ phys_list n (to_mnp_ptr node IsPtr) (val::L), n⟧)%I with "[Phys]" as "Phys".
-      { iApply phys_list_fold. simpl. des. iExists _,_. iFrame "∗#". done. }
+      destruct node as [|node]; [done|].
+      iAssert (⟦ phys_list n (Ptr node) (val::L), n⟧)%I with "[Phys]" as "Phys".
+      { iApply phys_list_fold. iExists _. iFrame "∗#". }
 
       (* Update liveness invariant *)
       iDestruct (LInv_unfold with "LInv") as "[GMap LivC]".
@@ -360,7 +361,7 @@ Section SPEC.
 
       (** Add it to the invariant. *)
       iDestruct (big_sepM_delete with "LivC") as "[_ LivC]"; [apply Lookup_i|].
-      iDestruct (LInv_fold _ _ _ (to_mnp_ptr node IsPtr) with "GMap [LivC Ob_ks]") as "LInv".
+      iDestruct (LInv_fold _ _ _ (Ptr node) with "GMap [LivC Ob_ks]") as "LInv".
       { iDestruct (big_sepM_sep_2 with "LivC Ob_ks") as "LivC".
         iApply (big_sepM_mono with "LivC").
         iIntros (i' p' Lookup_i') "[H C]". des_ifs.
@@ -387,10 +388,7 @@ Section SPEC.
     iIntros (b) "POST".
     iDestruct "POST" as (u) "(%EQ & s↦ & _ & _)".
     des_ifs. all: destruct EQ as [-> ->].
-    { exfalso. clear - e NEQ. unfold to_val in e.
-      destruct h as [h Ph],h' as [h' Ph']. simpl in *. clarify.
-      assert (Ph = Ph') as -> by apply proof_irrelevance. done.
-    }
+    { exfalso. clear - e NEQ. unfold to_val in e. des_ifs. }
 
     (* Update ◇[k](0,1) to use for induction *)
     iDestruct (LInv_unfold with "LInv") as "[GMap LivC]".
@@ -412,6 +410,7 @@ Section SPEC.
     iMod (pcs_drop _ _ 1 ltac:(auto) 1 98 with "[$Pcs]") as "Pcs"; [lia|].
     iMod ("IH" with "Ob_k n.n↦ Post Duty Pcs AU n.d↦ Ob_ks") as "IH".
     iApply "IH".
+    Local Transparent TreiberStack.push_loop.
   Qed.
 
   Lemma Treiber_pop_spec
@@ -436,10 +435,12 @@ Section SPEC.
             end
             )%S, 1+n⟧⧽
   .
-  Proof.
+  Proof using All.
     ii. iStartTriple. red_tl_all.
     unfold IsT,TStack. rewrite red_syn_tgt_interp_as. rewrite red_syn_atomic_update. red_tl. simpl.
-    iIntros "(#Mem & IsT & Duty & AU & Ob_ks & PCS) Post".
+    iIntros "(#Mem & IsT & Duty & AU & Ob_ks & PCS)".
+    set POST := (POST in (POST -∗ _)%I).
+    iIntros "Post".
     iDestruct "IsT" as (γl) "IsT".
     red_tl. rewrite red_syn_inv. iDestruct "IsT" as "#[Ob_kb IsT]".
 
@@ -465,7 +466,9 @@ Section SPEC.
         - iApply ("Ind" with "PCS").
     }
 
-    iModIntro. iExists 0. iIntros "IH !> PCS Post Duty Ys AU Ob_ks".
+    iModIntro. iExists 0.
+    set IH := (IH in (IH ==∗ _)%I).
+    iIntros "IH !> PCS Post Duty Ys AU Ob_ks".
     iEval (rewrite unfold_iter_eq). rred2r.
 
     iMod ((pcs_decr _ _ 100 1) with "Ys") as "[Ys Y]"; [lia|].
@@ -480,14 +483,11 @@ Section SPEC.
     subst. rred2r. iApply wpsim_tauR. rred2r.
     iMod ((pcs_decr _ _ 99 1) with "Ys") as "[Ys Y]"; [lia|].
 
-    destruct (decide (to_val h = to_mnp_null)) as [EQ|NEQ].
+    destruct (decide (h = Null)) as [->|NEQ].
     { (* Head is null, so stack is empty. *)
-      destruct h as [[h|h] EQh]; ss.
-      subst. injection EQ as ->. simpl in *.
+      simpl in *.
       iEval (rewrite phys_list_unfold) in "Phys".
-      des_ifs; last first.
-      { iDestruct "Phys" as (p r) "[%EQ _]". simpl in EQ. done. }
-      iClear "Phys".
+      des_ifs. iClear "Phys".
       iMod "AU" as (?) "[γs' Commit]". red_tl_all.
       iDestruct (ghost_var_agree with "γs γs'") as %<-.
       iMod ("Commit" $! tt with "γs'") as "Q".
@@ -506,8 +506,8 @@ Section SPEC.
           - iIntros "[$ _]".
         }
       1: lia.
-      iIntros (?) "%EQ". destruct EQ as [EQ _]. des; last done.
-      specialize (EQ EQh) as ->. rred2r.
+      iIntros (?) "%EQ". destruct EQ as [EQ _].
+      specialize (EQ ltac:(auto)) as ->. rred2r.
 
       iApply (wpsim_tauR). rred2r.
       iApply "Post". red_tl_all. iFrame.
@@ -562,9 +562,8 @@ Section SPEC.
       iDestruct (memory_ra_points_to_agree with "h.n↦□ h'.n↦□") as %<-.
 
       iDestruct (phys_list_unfold with "Phys") as "Phys".
-      destruct L as [|v tL].
-      { iDestruct "Phys" as %EQ. done. }
-      iDestruct "Phys" as (? r_new) "[%EQ_p [[#h.n↦□' [#h.d↦□' _]] Phys]]".
+      destruct L as [|v tL], h as [|[h]]; try done.
+      iDestruct "Phys" as (r_new) "[[#h.n↦□' [#h.d↦□' _]] Phys]".
 
       iDestruct (memory_ra_points_to_agree with "h.d↦□ h.d↦□'") as %<-.
       iDestruct (memory_ra_points_to_agree with "h.n↦□ h.n↦□'") as %->.
@@ -572,9 +571,7 @@ Section SPEC.
 
       (* Equal, CAS success *)
       iApply (SCMem_cas_loc_fun_spec_gen with "[$Mem $s↦] [-]"); [lia|solve_ndisj| |].
-      { des_ifs.
-        iSplit; iExists _; iFrame "h.n↦□".
-      }
+      { des_ifs. iSplit; iExists _; iFrame "h.n↦□". }
       iIntros (b) "POST".
 
       iDestruct "POST" as (u) "(%EQ & s↦ & _ & _)".
@@ -632,16 +629,14 @@ Section SPEC.
     (* Different, CAS fail *)
     iApply (SCMem_cas_loc_fun_spec_gen with "[$Mem $s↦ h.n↦□ h'↦□] [-]"); [lia|solve_ndisj| |].
     { unfold to_val. des_ifs.
-      2: iDestruct "h'↦□" as (??) "[h'↦□ _]".
+      2,4: iDestruct "h'↦□" as (??) "[h'↦□ _]".
       all: iSplit; try done; iExists _; iFrame "#".
     }
     iClear "h'↦□".
     iIntros (b) "POST". iDestruct "POST" as (u) "(%EQ & s↦ & _ & _)".
     destruct (SCMem.val_eq_dec (to_val h') (to_val h)).
     all: destruct EQ as [-> ->].
-    { exfalso. unfold to_val in e. apply NEQhh'.
-      destruct h,h'. simpl in *. subst. f_equal. apply proof_irrelevance.
-    }
+    { exfalso. unfold to_val in e. des_ifs. }
 
     (* Update ◇[k](0,1) to use for induction *)
     iDestruct (LInv_unfold with "LInv") as "[GMap LivC]".
